wip on top-level stateful API

pulse/share/steel/examples/pulse/dice/dpe/DPE.CBOR.fsti
@@ -11,30 +11,43 @@ module U8 = FStar.UInt8
 module A = Pulse.Lib.Array
 
 (* placeholder *)
-val parse_cbor (b:bytes) (#a:Type0) (x:a) : prop
+val parse_cbor (b:bytes) (#desc:cddl) (x:as_type desc) : prop
+
+let initialize_context_cddl =
+  [("sid", 0, UINT);
+   ("seed", 3, BYTES)]
+
+{
+   &(sid:0) => uint,
+   &(seed:3) => bytes,
+   *&(tstr:uint) => any
+}
 
 val initialize_context (len:SZ.t)
                        (input:A.larray U8.t (SZ.v len))
                        (len':SZ.t)
                        (output:A.larray U8.t (SZ.v len'))
+                       (#p:perm)
                        (#input_bytes:Ghost.erased bytes)
   : stt bool
     (requires
-      A.pts_to input input_bytes **
+      A.pts_to input #p input_bytes **
       exists_ (fun s -> A.pts_to output s))
     (ensures fun b ->
-      A.pts_to input input_bytes **
+      A.pts_to input #p input_bytes **
       exists_ (fun output_bytes -> 
         A.pts_to output output_bytes **
         (if not b
          then emp
          else (
-            exists_ (fun (sid:sid_t) ->
-            exists_ (fun (uds:bytes) ->
+            exists_ (fun (t:as_type initialize_context_cddl) ->
+            // exists_ (fun (sid:sid_t) ->
+            // exists_ (fun (uds:bytes) ->
             exists_ (fun (hndl:ctxt_hndl_t) ->
-                pure (parse_cbor input_bytes (sid, uds) /\
+                pure (parse_cbor input_bytes t /\ //(sid, uds) /\
                       parse_cbor output_bytes hndl) **
-                snapshot sid (EngineInitialized hndl uds)
+                snapshot (field_of t "sid")
+                         (EngineInitialized hndl (field_of t "seed"))
             )))
         ))))
         
